v1

tesis.dfy
@@ -12,7 +12,7 @@ datatype Condition =
   | Not(condition: Condition)
   | Imply(ConditonA: Condition, ConditonB: Condition) 
   | And(ConditonA: Condition, ConditonB: Condition) 
-  | Substitution(substitution: map<string, Expresion>)
+  | Substitution(substitution: map<string, Expresion>, condition: Condition)
   | Less(e1:Expresion, e2: Expresion)
   | Greater(e1:Expresion, e2: Expresion)
   | Equals(e1:Expresion, e2: Expresion)
@@ -20,8 +20,8 @@ datatype Condition =
 datatype Program =
   // | Skip // revisar
   | Assign(assignments: map<string, Expresion>)
-  | Secuence(instructions: Program, instruction: Program)
-  | If(condition: Condition, pThen: Program, pElse: Program,cp:Condition)
+  | Secuence(p1: Program, p2: Program)
+  | If(condition: Condition, pThen: Program, pElse: Program)
   | While(pInvariant: Condition, condition: Condition, body: Program)
 
 datatype Specification =
@@ -37,90 +37,127 @@ datatype THoare =
 //------------------------------------------------------------------------------------------------------
 //--------------------------------------- CORRECTNESS ---------------------------------------------------
 
-function Correctness (three: THoare): (Specification, set<Condition>){
-  match three
+// function Correctness (three: THoare): (Specification, set<Condition>){
+//   match three
 
-  case Assign(identifiers, condition) => (
-    Instruction(Condition.Substitution(identifiers),Program.Assign(identifiers),condition),{}
-  )
-  case If(condition, tree1, tree2,cp) => (
-      match Correctness(tree1)
+//   case Assign(identifiers, condition) => (
+//     Instruction(Condition.Substitution(identifiers),Program.Assign(identifiers),condition),{}
+//   )
+//   case If(condition, tree1, tree2,cp) => (
+//       match Correctness(tree1)
 
-      case (s1,cs1) =>
-      match s1
+//       case (s1,cs1) =>
+//       match s1
 
-      case Instruction(pc1, p1, c1) => 
-        match Correctness(tree2)
+//       case Instruction(pc1, p1, c1) => 
+//         match Correctness(tree2)
 
-        case (s2,cs2) => 
-          match s2
-          case Instruction(pc2, p2, c2) => (Instruction(And(Imply(condition,pc1),Imply(Not(condition),pc2)),Program.If(condition,p1,p2,cp),cp),(cs1 + cs2 + {Imply(pc1,cp),Imply(pc2,cp)})))
+//         case (s2,cs2) => 
+//           match s2
+//           case Instruction(pc2, p2, c2) => (Instruction(And(Imply(condition,pc1),Imply(Not(condition),pc2)),Program.If(condition,p1,p2,cp),cp),(cs1 + cs2 + {Imply(pc1,cp),Imply(pc2,cp)})))
   
-  case While(pInvariant, condition, tree) => (
-      match Correctness(tree)
+//   case While(pInvariant, condition, tree) => (
+//       match Correctness(tree)
 
-      case (s,cs) => 
-        match s
-        case Instruction(pc, p, c) => (Instruction(pInvariant,Program.While(pInvariant,condition,p),And(pInvariant,Not(condition))),cs + {Imply(And(pInvariant,condition),pc),Imply(c,pInvariant)}))
-  case Secuence(tree1, tree2) => (
-      match Correctness(tree1)
+//       case (s,cs) => 
+//         match s
+//         case Instruction(pc, p, c) => (Instruction(pInvariant,Program.While(pInvariant,condition,p),And(pInvariant,Not(condition))),cs + {Imply(And(pInvariant,condition),pc),Imply(c,pInvariant)}))
+//   case Secuence(tree1, tree2) => (
+//       match Correctness(tree1)
 
-      case (s1,cs1) => 
-        match s1
+//       case (s1,cs1) => 
+//         match s1
 
-        case Instruction(pc1, p1, c1) => 
-          match Correctness(tree2)
+//         case Instruction(pc1, p1, c1) => 
+//           match Correctness(tree2)
 
-          case (s2,cs2) => 
-            match s2
-            case Instruction(pc2, p2, c2) => (Instruction(pc1,Program.Secuence(p1,p2),c2),(cs1 + cs2 + {c1} + {pc2})))
+//           case (s2,cs2) => 
+//             match s2
+//             case Instruction(pc2, p2, c2) => (Instruction(pc1,Program.Secuence(p1,p2),c2),(cs1 + cs2 + {c1} + {pc2})))
 
-}
+// }
 
 //------------------------------------------------------------------------------------------------------
 //--------------------------------------- VCG ----------------------------------------------------------
 
-function VCG (specification: Specification): (THoare,set<Condition>){
+function VCG (specification: Specification): (multiset<Condition>){
   match specification
 
   case Instruction(precondition, program, postcondition) => (
     match VCGP(program,postcondition)
 
-    case (c,th,cs) => (
-      th,(cs + {Imply(precondition,postcondition)})
+    case (c,cs) => (
+      (cs + multiset{Imply(precondition,c)})
       )
     )
 
 }
 
-function VCGP (program: Program, postcondition: Condition): (Condition,THoare,set<Condition>){
+function VCGP (program: Program, postcondition: Condition): (Condition,multiset<Condition>)
+ensures var result := VCGP(program,postcondition) ; Hoare(Instruction(result.0,program,postcondition),result.1)
+decreases program
+{
   match program
-  case Assign(assignments) => (Condition.Substitution(assignments),THoare.Assign(assignments,postcondition),{})
-  case Secuence(instructions, instruction) => (
-    match VCGP(instructions, postcondition)
+  case Assign(assignments) => (Condition.Substitution(assignments,postcondition),multiset{})
+  case Secuence(p1, p2) => (
+    match VCGP(p2, postcondition)
 
-    case (c1,th1,cs1) => 
-      match VCGP(instruction, c1)
+    case (c1,cs1) => (
+      match VCGP(p1, c1)
 
-      case (c2,th2,cs2) => (c2,THoare.Secuence(th1,th2),cs1 + cs2))
-  case If(condition, pThen, pElse,cp) => (
-    match VCGP(pThen, postcondition)
+      case (c2,cs2) => assert Hoare(Instruction(c2, p1, c1), cs2); assert Hoare(Instruction(c1, p2, postcondition), cs1); (c2,cs2 + cs1)))
+      
+  case If(condition, p1, p2) => (
+    match VCGP(p1, postcondition)
 
-    case (c1,th1,cs1) => 
-      match VCGP(pElse, postcondition)
+    case (c1,cs1) => 
+      match VCGP(p2, postcondition)
 
-      case (c2,th2,cs2) => (And(Imply(condition,c1),Imply(Not(condition),c2)),THoare.If(condition,th1,th2,cp),cs1 + cs2)
+      case (c2,cs2) => var q := And(Imply(condition,c1),Imply(Not(condition),c2)); 
+      assert Hoare(Instruction(And(q, condition), p1, postcondition), cs1 + multiset{Imply(And(q, condition),c1)});
+      assert Hoare(Instruction(And(q, Not(condition)), p2, postcondition), cs2 + multiset{Imply(And(q, Not(condition)),c2)});
+      (q,(cs1 + multiset{Imply(And(q,condition),c1)}) + (cs2 + multiset{Imply(And(q,Not(condition)),c2)}))
       )
   case While(pInvariant, condition, body) => (
     match VCGP(body, pInvariant)
 
-    case (c,th,cs) => (pInvariant,THoare.While(pInvariant,condition,th),cs + {Imply(And(pInvariant,condition),c),Imply(And(pInvariant,Not(condition)),postcondition)})
+    case (c,cs) => (
+      pInvariant,
+      cs + multiset{
+        Imply(And(pInvariant,condition),c)
+        } +
+        multiset{
+        Imply(And(pInvariant,Not(condition)),postcondition)
+        }
+        )
     )
 }
 
 
-lemma VCGCorrectness(specification: Specification)
+ghost predicate Hoare(prog: Specification, vcs: multiset<Condition>)
+
+decreases var Instruction(precondition, program, postcondition)  := prog ; program, |vcs|
+
 {
-  var (vcgResult, cs) := VCG(specification);
-  assert Correctness(vcgResult) == (specification, cs);
+  (match prog
+  case Instruction(precondition, program, postcondition) => (
+    match program
+    case Assign(assignments) => (
+      precondition == Condition.Substitution(assignments,postcondition) && vcs == multiset{}
+    )
+    case Secuence(p1, p2) => (
+      exists s,vcs1,vcs2 :: Hoare(Instruction(precondition, p1, s), vcs1) && Hoare(Instruction(s, p2, postcondition), vcs2) && vcs == vcs1 + vcs2
+    )
+    case If(condition, p1, p2) => (
+      exists vcs1,vcs2 :: Hoare(Instruction(And(precondition,condition), p1, postcondition), vcs1) && 
+      Hoare(Instruction(And(precondition,Not(condition)), p2, postcondition), vcs2) && vcs == vcs1 + vcs2
+    )
+    case While(inv, b, p) => (
+       Hoare(Instruction(And(inv,b),p,inv),vcs) && (precondition == inv) && (postcondition == And(inv,Not(b)))
+    )
+  )
+  || (exists qP,vcs1 :: vcs == vcs1 + multiset{Imply(precondition,qP)} && assert |vcs1| < |vcs|; Hoare(Instruction(qP,program,postcondition),vcs1))
+  || (exists rP,vcs1 :: vcs == vcs1 + multiset{Imply(rP,postcondition)} && assert |vcs1| < |vcs|;Hoare(Instruction(precondition,program,rP),vcs1))
+  )
+  
 }
